fix up fomega

Fomega/Algorithm.lean
@@ -1,33 +1,141 @@
 
+import Fomega.Proof
 import Fomega.Basic
 
 namespace Fomega
 
-  inductive AlgorithmKind where
-  | check | cinfer | infer | wf
-
   @[simp]
-  abbrev CheckArgs : AlgorithmKind -> Type
-  | .check => Term × Term
-  | .cinfer => Term
-  | .infer => Term
+  abbrev CheckArgs : JudgmentVariant -> Type
+  | .prf => Term
   | .wf => Unit
 
   @[simp]
-  abbrev CheckRets : AlgorithmKind -> Type
-  | .check => Option Unit
-  | .cinfer => Option Term
-  | .infer => Option Term
+  abbrev CheckRets : JudgmentVariant -> Type
+  | .prf => Option Term
   | .wf => Option Unit
 
-  def check : (k : AlgorithmKind) -> Ctx Term -> CheckArgs k -> CheckRets k
+  partial def normalize : Term -> Term := by sorry
+
+  def is_kind : Term -> Option Const := by sorry
+
+  def is_type : Term -> Option Unit := by sorry
+
+  def is_dom : Const -> Const -> Option Unit := by sorry
+
+  def is_pi : Term -> Option (Term × Term) := by sorry
+
+  def is_times : Term -> Option (Term × Term) := by sorry
+
+  def is_unit : Term -> Option Unit := by sorry
+
+  def conv : Term -> Term -> Option Unit := by sorry
+
+  def check_witness : (k : JudgmentVariant) -> Ctx Term -> CheckArgs k -> CheckRets k
+  | .wf, _, () => .some .unit
+  | .prf, _, t => .some t
+
+  instance inst_Inhabited_check_def : Inhabited ((k : JudgmentVariant) -> Ctx Term -> CheckArgs k -> CheckRets k) where
+    default := check_witness
+
+  @[simp]
+  def check : (k : JudgmentVariant) -> Ctx Term -> CheckArgs k -> CheckRets k
   | .wf, [], () => .some .unit
   | .wf, .cons A Γ, () => do
-    let Ak <- check .infer Γ A
+    let Ak <- check .prf Γ A
     let _ <- check .wf Γ ()
-  | .infer, Γ, Π[A] B => sorry
-  | .check, _, _ => .none
-  | .cinfer, _, _ => .none
-  | .infer, _, _ => .none
+    let _ <- is_kind Ak
+    .some ()
+  | .prf, _, □ => .none
+  | .prf, Γ, ★ => do
+    let _ <- check .wf Γ ()
+    .some □
+  | .prf, Γ, #x => do
+    let _ <- check .wf Γ ()
+    .some (Γ d@ x)
+  | .prf, Γ, Π[A] B => do
+    let Ak <- check .prf Γ A
+    let Ak <- is_kind Ak
+    let Bk <- check .prf (A::Γ) B
+    let Bk <- is_kind Bk
+    let _ <- is_dom Ak Bk
+    .some (.const Bk)
+  | .prf, Γ, `λ[A] t => do
+    let Ak <- check .prf Γ A
+    let Ak <- is_kind Ak
+    let B <- check .prf (A::Γ) t
+    let Bk <- check .prf (A::Γ) B
+    let Bk <- is_kind Bk
+    let _ <- is_dom Ak Bk
+    .some (Π[A] B)
+  | .prf, Γ, f `@ a => do
+    let T <- check .prf Γ f
+    let (A, B) <- is_pi T
+    let A' <- check .prf Γ a
+    let _ <- conv A A'
+    .some (B β[a])
+  | .prf, Γ , A ⊗ B => do
+    let Ak <- check .prf Γ A
+    let _ <- is_type Ak
+    let Bk <- check .prf Γ B
+    let _ <- is_type Bk
+    .some ★
+  | .prf, Γ, (.pair t s) => do
+    let A <- check .prf Γ t
+    let Ak <- check .prf Γ A
+    let _ <- is_type Ak
+    let B <- check .prf Γ s
+    let Bk <- check .prf Γ B
+    let _ <- is_type Bk
+    .some (A ⊗ B)
+  | .prf, Γ, (.fst t) => do
+    let T <- check .prf Γ t
+    let (A, _) <- is_times T
+    .some A
+  | .prf, Γ, (.snd t) => do
+    let T <- check .prf Γ t
+    let (_, B) <- is_times T
+    .some B
+  | .prf, Γ, .unit_ty => do
+    let _ <- check .wf Γ ()
+    .some ★
+  | .prf, Γ, .unit => do
+    let _ <- check .wf Γ ()
+    .some (U)
+  | .prf, Γ, (.unit_rec d u t) => do
+    let _ <- check .prf Γ d
+    let T <- check .prf Γ u
+    let _ <- is_unit T
+    let A <- check .prf Γ t
+    let Ak <- check .prf Γ A
+    let _ <- is_type Ak
+    .some A
+  decreasing_by
+    repeat sorry
+
+  @[simp]
+  abbrev CheckSoundType (Γ : Ctx Term) : (v : JudgmentVariant) -> CheckArgs v -> CheckRets v -> Prop
+  | .prf => λ t r => ∀ A, r = .some A -> Γ ⊢ t : A
+  | .wf => λ _ r => r = .some () -> ⊢ Γ
+
+  theorem check_sound : check v Γ t = r -> CheckSoundType Γ v t r := by
+  intro h
+  induction v, Γ, t, r using check.induct <;> simp at *
+  case _ => intro h2; constructor
+  case _ ih1 ih2 =>
+    intro h1; subst h1
+    sorry
+  case _ => sorry
+  case _ => sorry
+  case _ => sorry
+  case _ => sorry
+  case _ => sorry
+  case _ => sorry
+  case _ => sorry
+  case _ => sorry
+  case _ => sorry
+  case _ => sorry
+  case _ => sorry
+  case _ => sorry
+  case _ => sorry
 
 end Fomega
