Fomega/Reduction.lean
@@ -3,12 +3,13 @@ import Common.Reduction
 
 inductive Red : Term -> Term -> Prop where
 -- Steps
-| beta : Red ((`λ b) `@ t) (b β[t])
+| beta : Red ((`λ[A] b) `@ t) (b β[t])
 | fst : Red ((Term.pair t s).fst) t
 | snd : Red ((Term.pair t s).snd) s
-| unit_rec : Red (.unit_rec (u) t) t
+| unit_rec : Red (.unit_rec d (u) t) t
 -- Congruences
-| lam_congr : Red t t' -> Red (.lam t) (.lam t')
+| lam_congr1 : Red A A' -> Red (.lam A t) (.lam A' t)
+| lam_congr2 : Red t t' -> Red (.lam A t) (.lam A t')
 | app_congr1 : Red f f' -> Red (.app f t) (.app f' t)
 | app_congr2 : Red t t' -> Red (.app f t) (.app f t')
 | all_congr1 : Red A A' -> Red (.all A B) (.all A' B)
@@ -19,24 +20,29 @@ inductive Red : Term -> Term -> Prop where
 | snd_congr : Red t t' -> Red (.snd t) (.snd t')
 | times_congr1 : Red A A' -> Red (.times A B) (.times A' B)
 | times_congr2 : Red B B' -> Red (.times A B) (.times A B')
-| unit_rec_congr1 : Red t1 t1' -> Red (.unit_rec t1 t2) (.unit_rec t1' t2)
-| unit_rec_congr2 : Red t2 t2' -> Red (.unit_rec t1 t2) (.unit_rec t1 t2')
+| unit_rec_congr1 : Red t1 t1' -> Red (.unit_rec t1 t2 t3) (.unit_rec t1' t2 t3)
+| unit_rec_congr2 : Red t2 t2' -> Red (.unit_rec t1 t2 t3) (.unit_rec t1 t2' t3)
+| unit_rec_congr3 : Red t3 t3' -> Red (.unit_rec t1 t2 t3) (.unit_rec t1 t2 t3')
 
 inductive ParRed : Term -> Term -> Prop where
 -- Steps
-| beta : ParRed b b' -> ParRed t t' -> ParRed ((`λ b) `@ t) (b' β[t'])
+| beta : ParRed b b' -> ParRed t t' -> ParRed ((`λ[A] b) `@ t) (b' β[t'])
 | fst : ParRed t t' -> ParRed s s' -> ParRed ((Term.pair t s).fst) t'
 | snd : ParRed t t' -> ParRed s s' -> ParRed ((Term.pair t s).snd) s'
-| unit_rec : ParRed t t' -> ParRed (.unit_rec (u) t) t'
+| unit_rec : ParRed t t' -> ParRed (.unit_rec d (u) t) t'
 -- Congruences
-| lam_congr : ParRed t t' -> ParRed (.lam t) (.lam t')
+| lam_congr : ParRed A A' -> ParRed t t' -> ParRed (.lam A t) (.lam A' t')
 | app_congr : ParRed f f' -> ParRed t t' -> ParRed (.app f t) (.app f' t')
 | all_congr : ParRed A A' -> ParRed B B' -> ParRed (.all A B) (.all A' B')
 | pair_congr : ParRed t t' -> ParRed s s' -> ParRed (.pair t s) (.pair t' s')
 | fst_congr : ParRed t t' -> ParRed (.fst t) (.fst t')
 | snd_congr : ParRed t t' -> ParRed (.snd t) (.snd t')
 | times_congr : ParRed A A' -> ParRed B B' -> ParRed (.times A B) (.times A' B')
-| unit_rec_congr : ParRed t1 t1' -> ParRed t2 t2' -> ParRed (.unit_rec t1 t2) (.unit_rec t1' t2')
+| unit_rec_congr :
+  ParRed t1 t1' ->
+  ParRed t2 t2' ->
+  ParRed t3 t3' ->
+  ParRed (.unit_rec t1 t2 t3) (.unit_rec t1' t2' t3')
 | var : ParRed (.var x) (.var x)
 | const : ParRed (.const k) (.const k)
 | unit : ParRed .unit .unit
@@ -45,11 +51,11 @@ inductive ParRed : Term -> Term -> Prop where
 namespace Term
   @[simp]
   def compl : Term -> Term
-  | app (lam b) t => (compl b) β[compl t]
+  | app (lam _ b) t => (compl b) β[compl t]
   | fst (pair t _) => compl t
   | snd (pair _ s) => compl s
-  | unit_rec (u) t => compl t
-  | lam t => lam (compl t)
+  | unit_rec _ (u) t => compl t
+  | lam A t => lam (compl A) (compl t)
   | app f a => app (compl f) (compl a)
   | all A B => all (compl A) (compl B)
   | pair t s => pair (compl t) (compl s)
@@ -58,7 +64,7 @@ namespace Term
   | snd t => snd (compl t)
   | unit => unit
   | unit_ty => unit_ty
-  | unit_rec t1 t2 => unit_rec (compl t1) (compl t2)
+  | unit_rec t1 t2 t3 => unit_rec (compl t1) (compl t2) (compl t3)
   | var n => var n
   | const K => const K
 end Term
@@ -82,8 +88,8 @@ namespace ParRed
   intro h; induction h generalizing σ <;> simp
   any_goals try apply red_refl
   any_goals try constructor <;> simp [*]
-  case _ b b' t t' _ _ ih1 ih2 =>
-    have lem : (`λ([^σ]b) `@ ([σ]t)) =β> ([^σ]b') β[[σ]t'] := by
+  case _ b b' t t' A _ _ ih1 ih2 =>
+    have lem : (`λ[[σ]A] ([^σ]b) `@ ([σ]t)) =β> ([^σ]b') β[[σ]t'] := by
       apply ParRed.beta (ih1 ^σ) (ih2 _)
     simp at lem; apply lem
   case _ ih1 ih2 => apply ParRed.fst; apply ih1; apply ih2
@@ -99,22 +105,26 @@ namespace ParRed
   any_goals (solve | constructor)
   any_goals (solve | try case _ ih => constructor; apply ih _ _ h1 h2)
   any_goals (solve | try case _ ih1 ih2 => constructor; apply ih1 _ _ h1 h2; apply ih2 _ _ h1 h2)
-  case _ b b' t t' _ _ ih1 ih2 =>
-    have lem : (`λ([^σ]b) `@ ([σ]t)) =β> ([^τ]b') β[[τ]t'] := by
+  case _ b b' t t' A  _ _ ih1 ih2 =>
+    have lem : (`λ[[σ]A]([^σ]b) `@ ([σ]t)) =β> ([^τ]b') β[[τ]t'] := by
       apply ParRed.beta
       replace ih1 := ih1 (^σ) (^τ) (Subst.lift_replace red_subst_same h1) (Subst.lift_rename h2)
       apply ih1; apply ih2 _ _ h1 h2
     simp at lem; apply lem
-  case _ t t' _ ih =>
-    have lem : `λ[^σ]t =β> `λ[^τ]t' := by
+  case _ A A' t t' _ _ ih1 ih2 =>
+    have lem : `λ[[σ]A][^σ]t =β> `λ[[τ]A'][^τ]t' := by
       constructor
-      apply ih (^σ) (^τ) (Subst.lift_replace red_subst_same h1) (Subst.lift_rename h2)
+      apply ih1 _ _ h1 h2
+      apply ih2 (^σ) (^τ) (Subst.lift_replace red_subst_same h1) (Subst.lift_rename h2)
     simp at lem; apply lem
   case _ A A' B B' _ _ ih1 ih2 =>
     have lem : Π[[σ]A][^σ]B =β> Π[[τ]A'][^τ]B' := by
       constructor; apply ih1 _ _ h1 h2
       apply ih2 (^σ) (^τ) (Subst.lift_replace red_subst_same h1) (Subst.lift_rename h2)
     simp at lem; apply lem
+  case _ ih1 ih2 ih3 =>
+    constructor; apply ih1 _ _ h1 h2
+    apply ih2 _ _ h1 h2; apply ih3 _ _ h1 h2
   case _ x =>
     generalize udef : σ x = u
     cases u <;> simp at *
@@ -162,13 +172,13 @@ namespace ParRed
       case _ r1 r2 =>
         cases ih; case _ ih1 ih2 =>
           apply ParRed.snd; apply ih1; apply ih2
-  case _ t1 t1' t2 t2' r1 _ ih1 ih2 =>
-    cases t1 <;> simp at * <;> try (constructor <;> simp [*])
+  case _ t1 t1' t2 t2' t3 t3' _r1 r2 _r3 ih1 ih2 ih3 =>
+    cases t2 <;> simp at * <;> try (constructor <;> simp [*])
     case _ =>
-      cases t1'
-      any_goals (try cases r1)
+      cases t2'
+      any_goals (try cases r2)
       case _ =>
-        apply ParRed.unit_rec; apply ih2
+        apply ParRed.unit_rec; apply ih3
 
 end ParRed
 
