Fomega/Basic/Substitution.lean
@@ -94,9 +94,10 @@ namespace Fomega.Proof
     simp; constructor; apply ih h2 h3 j2
   case unit_ty ih =>
     simp; constructor; apply ih h2 h3 j2
-  case unit_rec ih1 ih2 ih3 =>
+  case unit_rec ih1 ih2 ih3 ih4 =>
     simp; constructor; apply ih1 h2 h3 j2
     apply ih2 h2 h3 j2; apply ih3 h2 h3 j2
+    apply ih4 h2 h3 j2
   case conv Γ' t' A' B K _j1 _j2 j3 ih1 ih2 =>
     constructor; apply ih1 h2 h3 j2; apply ih2 h2 h3 j2
     apply Red.Conv.subst_same j3
